start updating passification theory to support constant propagation

BoogieLang/Passification.thy
@@ -4,6 +4,8 @@ begin
 
 text \<open>Dependence of set U on variables D\<close>
 
+type_synonym passive_rel = "vname \<rightharpoonup> (vname + lit)"
+
 definition lookup_var_ty_match :: "'a absval_ty_fun \<Rightarrow> var_context \<Rightarrow> rtype_env \<Rightarrow> 'a nstate \<Rightarrow> vname \<Rightarrow> ty \<Rightarrow> bool"
   where "lookup_var_ty_match A \<Lambda> \<Omega> ns x \<tau> = (Option.map_option (type_of_val A) (lookup_var \<Lambda> ns x) = Some (instantiate \<Omega> \<tau>))"
 
@@ -22,10 +24,6 @@ lemma dependent_ext:
   using assms
   unfolding dependent_def
   by blast
-                                                                       
-fun local_nstate :: "'a named_state \<Rightarrow> 'a nstate"
-  where "local_nstate local_ns = 
-    \<lparr> old_global_state = Map.empty, global_state = Map.empty, local_state = local_ns, binder_state = Map.empty \<rparr>"
 
 definition set_red_cmd :: "'a absval_ty_fun \<Rightarrow> method_context \<Rightarrow> var_context \<Rightarrow> 'a fun_interp \<Rightarrow> rtype_env \<Rightarrow> cmd \<Rightarrow> 'a nstate set \<Rightarrow> 'a state set"
   where "set_red_cmd A M \<Lambda> \<Gamma> \<Omega> c N = {s. \<exists>n_s. n_s \<in> N \<and> A,M,\<Lambda>,\<Gamma>,\<Omega> \<turnstile> \<langle>c, Normal n_s\<rangle> \<rightarrow> s}"
@@ -60,10 +58,11 @@ proof (induction rule: red_expr_red_exprs.inducts)
 qed (auto intro: red_expr_red_exprs.intros)
 
 (* todo: old variables, constants *)
-inductive expr_rel :: "(vname \<rightharpoonup> vname) \<Rightarrow> expr \<Rightarrow> expr \<Rightarrow> bool" and 
- expr_list_rel :: "(vname \<rightharpoonup> vname) \<Rightarrow> expr list \<Rightarrow> expr list \<Rightarrow> bool"
+inductive expr_rel :: "passive_rel \<Rightarrow> expr \<Rightarrow> expr \<Rightarrow> bool" and 
+ expr_list_rel :: "passive_rel \<Rightarrow> expr list \<Rightarrow> expr list \<Rightarrow> bool"
   where    
-   Var_Rel: "R x1 = Some x2 \<Longrightarrow> expr_rel R (Var x1) (Var x2)"
+   Var_Rel: "R x1 = Some (Inl x2) \<Longrightarrow> expr_rel R (Var x1) (Var x2)"
+ | Var_Const_Rel: "R x1 = Some (Inr l) \<Longrightarrow> expr_rel R (Var x1) (Lit l)"
  | BVar_Rel: "expr_rel R (BVar i) (BVar i)"
  | Lit_Rel: "expr_rel R (Lit lit) (Lit lit)"
  | UnOp_Rel: "expr_rel R e1 e2 \<Longrightarrow> expr_rel R (UnOp uop e1) (UnOp uop e2)"
@@ -83,20 +82,29 @@ method expr_rel_tac uses R_def =
                        "expr_list_rel ?R ?es1 ?es2" \<Rightarrow> rule \<bar> 
                        "_" \<Rightarrow> fail)+
 
-definition rel_well_typed
-  where "rel_well_typed A \<Lambda> \<Omega> R ns = (\<forall> x y. R x = Some y \<longrightarrow> 
-           (\<exists>v \<tau>. lookup_var \<Lambda> ns x = Some v \<and> lookup_var_ty \<Lambda> x = Some \<tau> \<and> type_of_val A v = instantiate \<Omega> \<tau>))"
+
+definition rel_const_correct :: "var_context \<Rightarrow> passive_rel \<Rightarrow> 'a nstate \<Rightarrow> bool"
+  where "rel_const_correct \<Lambda> R ns = 
+           (\<forall> x l. R x = Some (Inr l) \<longrightarrow>
+            ( lookup_var \<Lambda> ns x = Some (LitV l) \<and> lookup_var_ty \<Lambda> x = Some (TPrim (type_of_lit l)) ))"
+
+definition rel_well_typed :: "'a absval_ty_fun \<Rightarrow> var_context \<Rightarrow> rtype_env \<Rightarrow> passive_rel \<Rightarrow> 'a nstate \<Rightarrow> bool"
+  where "rel_well_typed A \<Lambda> \<Omega> R ns = (
+           (\<forall> x y. R x = Some (Inl y) \<longrightarrow> 
+             (\<exists>v \<tau>. lookup_var \<Lambda> ns x = Some v \<and> lookup_var_ty \<Lambda> x = Some \<tau> \<and> type_of_val A v = instantiate \<Omega> \<tau>)) \<and>
+           (rel_const_correct \<Lambda> R ns))"
+
 
 lemma rel_well_typed_update: 
   assumes "rel_well_typed A \<Lambda> \<Omega> R ns" and "lookup_var_ty \<Lambda> x = Some \<tau>" and "type_of_val A v = instantiate \<Omega> \<tau>"
-  shows "rel_well_typed A \<Lambda> \<Omega> (R(x \<mapsto> x')) (update_var \<Lambda> ns x v)"
+  shows "rel_well_typed A \<Lambda> \<Omega> (R(x \<mapsto> (Inl x'))) (update_var \<Lambda> ns x v)"
   using assms
-  unfolding rel_well_typed_def
+  unfolding rel_well_typed_def rel_const_correct_def 
   by simp
 
-definition nstate_rel
+definition nstate_rel :: "var_context \<Rightarrow> var_context \<Rightarrow> passive_rel \<Rightarrow> 'a nstate \<Rightarrow> 'a nstate \<Rightarrow> bool"
   where "nstate_rel \<Lambda> \<Lambda>' R ns1 ns2 = 
-          ((\<forall>x y.  R x = Some y \<longrightarrow> (lookup_var \<Lambda> ns1 x = lookup_var \<Lambda>' ns2 y))
+          ((\<forall>x y.  R x = Some (Inl y) \<longrightarrow> (lookup_var \<Lambda> ns1 x = lookup_var \<Lambda>' ns2 y))
             \<and> binder_state ns1 = binder_state ns2)"
 
 definition nstate_rel_states
@@ -105,13 +113,13 @@ definition nstate_rel_states
 definition update_nstate_rel
   where "update_nstate_rel R upds  = R ((map fst upds) [\<mapsto>] (map snd upds))"
 
-lemma lookup_nstate_rel: "R x = Some y \<Longrightarrow> nstate_rel \<Lambda> \<Lambda>' R ns u \<Longrightarrow> rel_well_typed A \<Lambda> \<Omega> R ns \<Longrightarrow>
+lemma lookup_nstate_rel: "R x = Some (Inl y) \<Longrightarrow> nstate_rel \<Lambda> \<Lambda>' R ns u \<Longrightarrow> rel_well_typed A \<Lambda> \<Omega> R ns \<Longrightarrow>
    lookup_var \<Lambda>' u y = Some (the (lookup_var \<Lambda> ns x))"
   unfolding nstate_rel_def rel_well_typed_def
   using option.exhaust_sel by force  
 
 lemma lookup_nstates_rel: "u \<in> U \<Longrightarrow> nstate_rel_states \<Lambda> \<Lambda>' R ns U \<Longrightarrow>  rel_well_typed A \<Lambda> \<Omega> R ns \<Longrightarrow>
-           R x = Some y \<Longrightarrow> 
+           R x = Some (Inl y) \<Longrightarrow> 
            lookup_var \<Lambda>' u y = Some (the (lookup_var \<Lambda> ns x))"
   unfolding nstate_rel_states_def
   using lookup_nstate_rel by blast
@@ -119,10 +127,10 @@ lemma lookup_nstates_rel: "u \<in> U \<Longrightarrow> nstate_rel_states \<Lambd
 lemma update_var_nstate_rel:
   assumes Srel:"nstate_rel \<Lambda> \<Lambda>' R ns1 ns2" and
           "lookup_var \<Lambda>' ns2 x = Some v"
-  shows "nstate_rel \<Lambda> \<Lambda>' (R(y \<mapsto> x)) (update_var \<Lambda> ns1 y v) ns2" 
+  shows "nstate_rel \<Lambda> \<Lambda>' (R(y \<mapsto> (Inl x))) (update_var \<Lambda> ns1 y v) ns2" 
 proof (simp only: nstate_rel_def, rule conjI, rule allI, rule allI, rule impI)
   fix z1 z2
-  assume Map:"(R(y \<mapsto> x)) z1 = Some z2"
+  assume Map:"(R(y \<mapsto> (Inl x))) z1 = Some (Inl z2)"
   show "lookup_var \<Lambda> (update_var \<Lambda> ns1 y v) z1 = lookup_var \<Lambda>' ns2 z2"
   proof (cases "z1 = y")
     case True
@@ -146,14 +154,14 @@ lemma update_nstate_rel_nil: "update_nstate_rel R [] = R"
 
   
 lemma update_rel_nstate_same_state:
-  assumes Srel: "nstate_rel \<Lambda> \<Lambda>' R ns1 ns2" and "R x = Some x1" and LookupEq:"lookup_var \<Lambda>' ns2 x1 = lookup_var \<Lambda>' ns2 x2"
-  shows "nstate_rel \<Lambda> \<Lambda>' (R(x \<mapsto> x2)) ns1 ns2"
+  assumes Srel: "nstate_rel \<Lambda> \<Lambda>' R ns1 ns2" and "R x = Some (Inl x1)" and LookupEq:"lookup_var \<Lambda>' ns2 x1 = lookup_var \<Lambda>' ns2 x2"
+  shows "nstate_rel \<Lambda> \<Lambda>' (R(x \<mapsto> (Inl x2))) ns1 ns2"
 proof (unfold nstate_rel_def, rule+)
   fix arg y
-  assume "(R(x \<mapsto> x2)) arg = Some y"
+  assume "(R(x \<mapsto> (Inl x2))) arg = Some (Inl y)"
   thus "lookup_var \<Lambda> ns1 arg = lookup_var \<Lambda>' ns2 y"
-   using Srel \<open>R x = Some x1\<close> LookupEq
-   by (metis map_upd_Some_unfold nstate_rel_def)  
+   using Srel \<open>R x = Some (Inl x1)\<close> LookupEq
+   by (metis fun_upd_apply nstate_rel_def option.sel sum.inject(1))   
 next
   from Srel show "binder_state ns1 = binder_state ns2" by (simp add: nstate_rel_def)
 qed
@@ -161,14 +169,21 @@ qed
 lemma binder_update_nstate_rel: "nstate_rel \<Lambda> \<Lambda>' R ns1 ns2 \<Longrightarrow> (\<And>v. nstate_rel \<Lambda> \<Lambda>' R (full_ext_env ns1 v) (full_ext_env ns2 v))"
   unfolding nstate_rel_def
   apply (simp only: lookup_full_ext_env_same)
-  by (simp add: binder_full_ext_env_same)  
+  by (simp add: binder_full_ext_env_same)
+
+lemma binder_update_rel_const: "rel_const_correct \<Lambda> R ns \<Longrightarrow> (\<And>v. rel_const_correct \<Lambda> R (full_ext_env ns v))"
+  unfolding rel_const_correct_def
+  by (simp only: lookup_full_ext_env_same) auto    
 
 lemma expr_rel_same:
-  shows "expr_rel R e1 e2 \<Longrightarrow> nstate_rel \<Lambda> \<Lambda>' R ns1 ns2 \<Longrightarrow> A,\<Lambda>,\<Gamma>,\<Omega> \<turnstile> \<langle>e1, ns1\<rangle> \<Down> v \<Longrightarrow> A,\<Lambda>',\<Gamma>,\<Omega> \<turnstile> \<langle>e2, ns2\<rangle> \<Down> v" and
-    "expr_list_rel R es1 es2 \<Longrightarrow> nstate_rel \<Lambda> \<Lambda>' R ns1 ns2 \<Longrightarrow> A,\<Lambda>,\<Gamma>,\<Omega> \<turnstile> \<langle>es1, ns1\<rangle> [\<Down>] vs \<Longrightarrow> A,\<Lambda>',\<Gamma>,\<Omega> \<turnstile> \<langle>es2, ns2\<rangle> [\<Down>] vs" 
+  shows "expr_rel R e1 e2 \<Longrightarrow> rel_const_correct \<Lambda> R ns1 \<Longrightarrow> nstate_rel \<Lambda> \<Lambda>' R ns1 ns2 \<Longrightarrow> A,\<Lambda>,\<Gamma>,\<Omega> \<turnstile> \<langle>e1, ns1\<rangle> \<Down> v \<Longrightarrow> A,\<Lambda>',\<Gamma>,\<Omega> \<turnstile> \<langle>e2, ns2\<rangle> \<Down> v" and
+    "expr_list_rel R es1 es2 \<Longrightarrow> rel_const_correct \<Lambda> R ns1 \<Longrightarrow> nstate_rel \<Lambda> \<Lambda>' R ns1 ns2 \<Longrightarrow> A,\<Lambda>,\<Gamma>,\<Omega> \<turnstile> \<langle>es1, ns1\<rangle> [\<Down>] vs \<Longrightarrow> A,\<Lambda>',\<Gamma>,\<Omega> \<turnstile> \<langle>es2, ns2\<rangle> [\<Down>] vs" 
 proof (induction arbitrary: v ns1 ns2 \<Omega> and vs ns1 ns2 \<Omega> rule: expr_rel_expr_list_rel.inducts)
   case (Var_Rel R x1 x2)
   thus ?case  by (auto intro: red_expr_red_exprs.intros simp: nstate_rel_def)
+next
+  case (Var_Const_Rel R x1 l)
+  then show ?case by (auto intro: red_expr_red_exprs.intros simp: rel_const_correct_def)
 next
   case (BVar_Rel R x1 x2)
   thus ?case 
@@ -187,26 +202,28 @@ next
   then show ?case by (blast intro: red_expr_red_exprs.intros)
 next
   case (Forall_Rel R e1 e2 ty)
-  hence RelExt:"\<And>v. nstate_rel \<Lambda> \<Lambda>' R (full_ext_env ns1 v) (full_ext_env ns2 v)" using binder_update_nstate_rel by blast    
+  hence RelExt:"\<And>v. nstate_rel \<Lambda> \<Lambda>' R (full_ext_env ns1 v) (full_ext_env ns2 v)" using binder_update_nstate_rel by blast 
+  from Forall_Rel have RelWtExt:"\<And>v. rel_const_correct \<Lambda> R (full_ext_env ns1 v)" using binder_update_rel_const by blast 
   from \<open>A,\<Lambda>,\<Gamma>,\<Omega> \<turnstile> \<langle>Forall ty e1,ns1\<rangle> \<Down> v\<close>
   show ?case
-    by (cases; blast intro: red_expr_red_exprs.intros dest:Forall_Rel.IH[OF RelExt])
+  by (cases; blast intro: red_expr_red_exprs.intros dest:Forall_Rel.IH[OF RelWtExt RelExt])
 next
   case (Exists_Rel R e1 e2 ty)
-  hence RelExt:"\<And>v. nstate_rel \<Lambda> \<Lambda>' R (full_ext_env ns1 v) (full_ext_env ns2 v)" using binder_update_nstate_rel by blast    
+  hence RelExt:"\<And>v. nstate_rel \<Lambda> \<Lambda>' R (full_ext_env ns1 v) (full_ext_env ns2 v)" using binder_update_nstate_rel by blast
+  from Exists_Rel have RelWtExt:"\<And>v. rel_const_correct \<Lambda> R (full_ext_env ns1 v)" using binder_update_rel_const by blast 
   from \<open>A,\<Lambda>,\<Gamma>,\<Omega> \<turnstile> \<langle>Exists ty e1,ns1\<rangle> \<Down> v\<close>
   show ?case
-    by (cases; blast intro: red_expr_red_exprs.intros dest:Exists_Rel.IH[OF RelExt])
+    by (cases; blast intro: red_expr_red_exprs.intros dest:Exists_Rel.IH[OF RelWtExt RelExt])
 next
   case (ForallT_Rel R e1 e2)
   from \<open>A,\<Lambda>,\<Gamma>,\<Omega> \<turnstile> \<langle>ForallT e1,ns1\<rangle> \<Down> v\<close>
   show ?case
-    by cases (auto intro: red_expr_red_exprs.intros dest: ForallT_Rel.IH[OF \<open>nstate_rel \<Lambda> \<Lambda>' R ns1 ns2\<close>])
+    by cases (auto intro: red_expr_red_exprs.intros dest: ForallT_Rel.IH[OF \<open>rel_const_correct \<Lambda> R ns1\<close> \<open>nstate_rel \<Lambda> \<Lambda>' R ns1 ns2\<close>])
 next
   case (ExistsT_Rel R e1 e2)
   from \<open>A,\<Lambda>,\<Gamma>,\<Omega> \<turnstile> \<langle>ExistsT e1,ns1\<rangle> \<Down> v\<close>
   show ?case
-    by cases (auto intro: red_expr_red_exprs.intros dest: ExistsT_Rel.IH[OF \<open>nstate_rel \<Lambda> \<Lambda>' R ns1 ns2\<close>])
+    by cases (auto intro: red_expr_red_exprs.intros dest: ExistsT_Rel.IH[OF \<open>rel_const_correct \<Lambda> R ns1\<close> \<open>nstate_rel \<Lambda> \<Lambda>' R ns1 ns2\<close>])
 next
   case (Nil_Rel R)
   then show ?case
@@ -218,7 +235,7 @@ next
 qed
 
 lemma expr_rel_same_set:
-  assumes "expr_rel R e1 e2" and "A,\<Lambda>,\<Gamma>,\<Omega> \<turnstile> \<langle>e1, ns1\<rangle> \<Down> v" and "nstate_rel_states \<Lambda> \<Lambda>' R ns1 U" 
+  assumes "expr_rel R e1 e2" and "A,\<Lambda>,\<Gamma>,\<Omega> \<turnstile> \<langle>e1, ns1\<rangle> \<Down> v" and "rel_const_correct \<Lambda> R ns1" and "nstate_rel_states \<Lambda> \<Lambda>' R ns1 U"
   shows "\<forall>u \<in> U. A,\<Lambda>',\<Gamma>,\<Omega> \<turnstile> \<langle>e2, u\<rangle> \<Down> v"
   using assms expr_rel_same unfolding nstate_rel_states_def by blast
 
@@ -363,11 +380,11 @@ proof -
 qed
 
 lemma assume_sync_nstate_rel:
-  assumes "R x_orig = Some x1" and
+  assumes "R x_orig = Some (Inl x1)" and
           Srel:"nstate_rel_states \<Lambda> \<Lambda>' R ns U" and 
           Rel_wt: "rel_well_typed A \<Lambda> \<Omega> R ns"
-  shows "nstate_rel_states \<Lambda> \<Lambda>' (R(x_orig \<mapsto> x2)) ns {ns'. Normal ns' \<in> (set_red_cmd A M \<Lambda>' \<Gamma> \<Omega> (Assume ((Var x2) \<guillemotleft>Eq\<guillemotright> (Var x1))) U)}"
- (is "nstate_rel_states \<Lambda> \<Lambda>' (R(x_orig \<mapsto> x2)) ns ?U'")
+  shows "nstate_rel_states \<Lambda> \<Lambda>' (R(x_orig \<mapsto> (Inl x2))) ns {ns'. Normal ns' \<in> (set_red_cmd A M \<Lambda>' \<Gamma> \<Omega> (Assume ((Var x2) \<guillemotleft>Eq\<guillemotright> (Var x1))) U)}"
+ (is "nstate_rel_states \<Lambda> \<Lambda>' (R(x_orig \<mapsto> (Inl x2))) ns ?U'")
 proof (unfold nstate_rel_states_def, rule ballI)
   have Apassive:"isPassive (Assume ((Var x2) \<guillemotleft>Eq\<guillemotright> (Var x1)))" by simp
   fix u'
@@ -376,35 +393,36 @@ proof (unfold nstate_rel_states_def, rule ballI)
   with Srel have "nstate_rel \<Lambda> \<Lambda>' R ns u'" by (simp add: nstate_rel_states_def)
   let ?v = "(the (lookup_var \<Lambda> ns x_orig))"
   have "A,\<Lambda>',\<Gamma>,\<Omega> \<turnstile> \<langle>Var x1, u'\<rangle> \<Down> ?v"
-    using lookup_nstate_rel[OF \<open>R x_orig = Some x1\<close> \<open>nstate_rel \<Lambda> \<Lambda>' R ns u'\<close> Rel_wt]
+    using lookup_nstate_rel[OF \<open>R x_orig = Some (Inl x1)\<close> \<open>nstate_rel \<Lambda> \<Lambda>' R ns u'\<close> Rel_wt]
     by (auto intro: RedVar)
   hence Lookup1:"lookup_var \<Lambda>' u' x1 = Some ?v" by auto
   from \<open>u' \<in> ?U'\<close> have "A,\<Lambda>',\<Gamma>,\<Omega> \<turnstile> \<langle>Var x2, u'\<rangle> \<Down> ?v" 
    using  expr_eval_determ(1)[OF \<open>A,\<Lambda>',\<Gamma>,\<Omega> \<turnstile> \<langle>Var x1, u'\<rangle> \<Down> ?v\<close>] assume_reduction_args by metis
   hence "lookup_var \<Lambda>' u' x2 = Some ?v" by auto
-  thus "nstate_rel \<Lambda> \<Lambda>' (R(x_orig \<mapsto> x2)) ns u'"
-    using Lookup1 update_rel_nstate_same_state[OF \<open>nstate_rel \<Lambda> \<Lambda>' R ns u'\<close> \<open>R x_orig = Some x1\<close>] 
+  thus "nstate_rel \<Lambda> \<Lambda>' (R(x_orig \<mapsto> (Inl x2))) ns u'"
+    using Lookup1 update_rel_nstate_same_state[OF \<open>nstate_rel \<Lambda> \<Lambda>' R ns u'\<close> \<open>R x_orig = Some (Inl x1)\<close>] 
     by simp
 qed
 
 lemma assume_assign_nstate_rel:
   assumes Erel:"expr_rel R e1 e2" and
           "A,\<Lambda>,\<Gamma>,\<Omega> \<turnstile> \<langle>e1, ns\<rangle> \<Down> v" and
-          Srel:"nstate_rel_states \<Lambda> \<Lambda>' R ns U"
+          Srel:"nstate_rel_states \<Lambda> \<Lambda>' R ns U" and 
+          Crel:"rel_const_correct \<Lambda> R ns"
   shows   "nstate_rel_states 
-               \<Lambda> \<Lambda>' (R(x_orig \<mapsto> x)) (update_var \<Lambda> ns x_orig v) {ns'. Normal ns' \<in> (set_red_cmd A M \<Lambda>' \<Gamma> \<Omega> (Assume ((Var x) \<guillemotleft>Eq\<guillemotright> e2)) U)}" 
- (is "nstate_rel_states \<Lambda> \<Lambda>' (R(x_orig \<mapsto> x)) (update_var \<Lambda> ns x_orig v) ?U'")
+               \<Lambda> \<Lambda>' (R(x_orig \<mapsto> (Inl x))) (update_var \<Lambda> ns x_orig v) {ns'. Normal ns' \<in> (set_red_cmd A M \<Lambda>' \<Gamma> \<Omega> (Assume ((Var x) \<guillemotleft>Eq\<guillemotright> e2)) U)}" 
+ (is "nstate_rel_states \<Lambda> \<Lambda>' (R(x_orig \<mapsto> (Inl x))) (update_var \<Lambda> ns x_orig v) ?U'")
 proof (unfold nstate_rel_states_def, rule ballI)
   have Apassive:"isPassive (Assume ((Var x) \<guillemotleft>Eq\<guillemotright> e2))" by simp
   fix u'
   assume "u' \<in> ?U'"
   hence "u' \<in> U" using passive_states_subset[OF Apassive] by blast
   with Srel have "nstate_rel \<Lambda> \<Lambda>' R ns u'" by (simp add: nstate_rel_states_def)
-  have "A,\<Lambda>',\<Gamma>,\<Omega> \<turnstile> \<langle>e2, u'\<rangle> \<Down> v" using expr_rel_same(1)[OF Erel \<open>nstate_rel \<Lambda> \<Lambda>' R ns u'\<close> \<open>A,\<Lambda>,\<Gamma>,\<Omega> \<turnstile> \<langle>e1, ns\<rangle> \<Down> v\<close>] by simp
+  have "A,\<Lambda>',\<Gamma>,\<Omega> \<turnstile> \<langle>e2, u'\<rangle> \<Down> v" using expr_rel_same(1)[OF Erel Crel \<open>nstate_rel \<Lambda> \<Lambda>' R ns u'\<close> \<open>A,\<Lambda>,\<Gamma>,\<Omega> \<turnstile> \<langle>e1, ns\<rangle> \<Down> v\<close>] by simp
   from \<open>u' \<in> ?U'\<close> have "A,\<Lambda>',\<Gamma>,\<Omega> \<turnstile> \<langle>Var x, u'\<rangle> \<Down> v" 
      using  expr_eval_determ(1)[OF \<open>A,\<Lambda>',\<Gamma>,\<Omega> \<turnstile> \<langle>e2, u'\<rangle> \<Down> v\<close>] assume_reduction_args by metis
   hence "lookup_var \<Lambda>' u' x = Some v" by auto
-  from this show "nstate_rel \<Lambda> \<Lambda>' (R(x_orig \<mapsto> x)) (update_var \<Lambda> ns x_orig v) u'" 
+  from this show "nstate_rel \<Lambda> \<Lambda>' (R(x_orig \<mapsto> (Inl x))) (update_var \<Lambda> ns x_orig v) u'" 
     by (rule update_var_nstate_rel[OF \<open>nstate_rel \<Lambda> \<Lambda>' R ns u'\<close>])
 qed
 
@@ -420,32 +438,35 @@ lemma single_assign_reduce_2:
 lemma assume_rel_normal:
   assumes Ared:"A,\<Lambda>,\<Gamma>,\<Omega> \<turnstile> \<langle>e1, ns\<rangle> \<Down> (BoolV True)" and
           Srel:"nstate_rel_states \<Lambda> \<Lambda>' R ns U" and 
+          Crel:"rel_const_correct \<Lambda> R ns" and
           Erel:"expr_rel R e1 e2"
         shows "\<And>u. u \<in> U \<Longrightarrow> A,M,\<Lambda>',\<Gamma>,\<Omega> \<turnstile> \<langle>Assume e2, Normal u\<rangle> \<rightarrow> Normal u"
 proof -
   fix u
   assume "u \<in> U"
   with Srel have "nstate_rel \<Lambda> \<Lambda>' R ns u" by (simp add: nstate_rel_states_def)
-  with Ared Erel have "A,\<Lambda>',\<Gamma>,\<Omega> \<turnstile> \<langle>e2, u\<rangle> \<Down> (BoolV True)" using expr_rel_same by blast
+  with Ared Erel have "A,\<Lambda>',\<Gamma>,\<Omega> \<turnstile> \<langle>e2, u\<rangle> \<Down> (BoolV True)" using expr_rel_same Crel by blast
   thus "A,M,\<Lambda>',\<Gamma>,\<Omega> \<turnstile> \<langle>Assume e2,Normal u\<rangle> \<rightarrow> Normal u" by (auto intro: RedAssumeOk)
 qed
 
 lemma assume_rel_magic:
   assumes Ared:"A,\<Lambda>,\<Gamma>,\<Omega> \<turnstile> \<langle>e1, ns\<rangle> \<Down> (BoolV False)" and
-          Srel:"nstate_rel_states \<Lambda> \<Lambda>' R ns U" and 
+          Srel:"nstate_rel_states \<Lambda> \<Lambda>' R ns U" and
+          Crel:"rel_const_correct \<Lambda> R ns" and
           Erel:"expr_rel R e1 e2"
   shows "\<And>u. u \<in> U \<Longrightarrow> A,M,\<Lambda>',\<Gamma>,\<Omega> \<turnstile> \<langle>Assume e2, Normal u\<rangle> \<rightarrow> Magic"
 proof -
   fix u
   assume "u \<in> U"
   with Srel have "nstate_rel \<Lambda> \<Lambda>' R ns u" by (simp add: nstate_rel_states_def)
-  with Ared Erel have "A,\<Lambda>',\<Gamma>,\<Omega> \<turnstile> \<langle>e2, u\<rangle> \<Down> (BoolV False)" using expr_rel_same by blast
+  with Ared Erel have "A,\<Lambda>',\<Gamma>,\<Omega> \<turnstile> \<langle>e2, u\<rangle> \<Down> (BoolV False)" using expr_rel_same Crel by blast
   thus "A,M,\<Lambda>',\<Gamma>,\<Omega> \<turnstile> \<langle>Assume e2,Normal u\<rangle> \<rightarrow> Magic" by (auto intro: RedAssumeMagic)
 qed
 
 lemma assert_rel_normal:
   assumes Ared:"A,\<Lambda>,\<Gamma>,\<Omega> \<turnstile> \<langle>e1, ns\<rangle> \<Down> (BoolV True)" and
           Srel:"nstate_rel_states \<Lambda> \<Lambda>' R ns U" and 
+          Crel:"rel_const_correct \<Lambda> R ns" and
           Erel:"expr_rel R e1 e2"
   shows "{ns'. Normal ns' \<in> (set_red_cmd A M \<Lambda>' \<Gamma> \<Omega> (Assert e2) U)} = U" (is "?U' = U")
 proof 
@@ -457,7 +478,7 @@ next
     fix u
     assume "u \<in> U"
     with Srel have "nstate_rel \<Lambda> \<Lambda>' R ns u" by (simp add: nstate_rel_states_def)
-    with Ared Erel have "A,\<Lambda>',\<Gamma>,\<Omega> \<turnstile> \<langle>e2, u\<rangle> \<Down> (BoolV True)" using expr_rel_same by blast
+    with Ared Erel have "A,\<Lambda>',\<Gamma>,\<Omega> \<turnstile> \<langle>e2, u\<rangle> \<Down> (BoolV True)" using expr_rel_same Crel by blast
     with \<open>u \<in> U\<close> show "u \<in> ?U'"
       by (auto intro!: red_cmd.intros simp: set_red_cmd_def)
   qed
@@ -465,36 +486,38 @@ qed
 
 lemma assert_rel_normal_2:
   assumes Ared:"A,\<Lambda>,\<Gamma>,\<Omega> \<turnstile> \<langle>e1, ns\<rangle> \<Down> (BoolV True)" and
-          Srel:"nstate_rel_states \<Lambda> \<Lambda>' R ns U" and 
+          Srel:"nstate_rel_states \<Lambda> \<Lambda>' R ns U" and
+          Crel:"rel_const_correct \<Lambda> R ns" and
           Erel:"expr_rel R e1 e2"
         shows "\<And>u. u \<in> U \<Longrightarrow> A,M,\<Lambda>',\<Gamma>,\<Omega> \<turnstile> \<langle>Assert e2, Normal u\<rangle> \<rightarrow> Normal u"
 proof -
   fix u
   assume "u \<in> U"
   with Srel have "nstate_rel \<Lambda> \<Lambda>' R ns u" by (simp add: nstate_rel_states_def)
-  with Ared Erel have "A,\<Lambda>',\<Gamma>,\<Omega> \<turnstile> \<langle>e2, u\<rangle> \<Down> (BoolV True)" using expr_rel_same by blast
+  with Ared Erel have "A,\<Lambda>',\<Gamma>,\<Omega> \<turnstile> \<langle>e2, u\<rangle> \<Down> (BoolV True)" using expr_rel_same Crel by blast
   thus "A,M,\<Lambda>',\<Gamma>,\<Omega> \<turnstile> \<langle>Assert e2,Normal u\<rangle> \<rightarrow> Normal u" by (auto intro: RedAssertOk)
 qed
 
 lemma assert_rel_failure:
   assumes Ared:"A,\<Lambda>,\<Gamma>,\<Omega> \<turnstile> \<langle>e1, ns\<rangle> \<Down> (BoolV False)" and
           Srel:"nstate_rel_states \<Lambda> \<Lambda>' R ns U" and 
+          Crel:"rel_const_correct \<Lambda> R ns" and
           Erel:"expr_rel R e1 e2"
   shows "\<And>u. u \<in> U \<Longrightarrow> A,M,\<Lambda>',\<Gamma>,\<Omega> \<turnstile> \<langle>Assert e2, Normal u\<rangle> \<rightarrow> Failure"
 proof -
   fix u
   assume "u \<in> U"
   with Srel have "nstate_rel \<Lambda> \<Lambda>' R ns u" by (simp add: nstate_rel_states_def)
-  with Ared Erel have "A,\<Lambda>',\<Gamma>,\<Omega> \<turnstile> \<langle>e2, u\<rangle> \<Down> (BoolV False)" using expr_rel_same by blast
+  with Ared Erel have "A,\<Lambda>',\<Gamma>,\<Omega> \<turnstile> \<langle>e2, u\<rangle> \<Down> (BoolV False)" using expr_rel_same Crel by blast
   thus "A,M,\<Lambda>',\<Gamma>,\<Omega> \<turnstile> \<langle>Assert e2,Normal u\<rangle> \<rightarrow> Failure" by (auto intro: RedAssertFail)
 qed
 
 lemma havoc_nstate_rel:
   assumes Srel:"nstate_rel_states \<Lambda> \<Lambda>' R ns U"
   shows   "nstate_rel_states 
-               \<Lambda> \<Lambda>' (R(x_orig \<mapsto> x2)) (update_var \<Lambda> ns x_orig v) {u' \<in> U. lookup_var \<Lambda>' u' x2 = Some v}"
+               \<Lambda> \<Lambda>' (R(x_orig \<mapsto> (Inl x2))) (update_var \<Lambda> ns x_orig v) {u' \<in> U. lookup_var \<Lambda>' u' x2 = Some v}"
  (is "nstate_rel_states 
-               \<Lambda> \<Lambda>' (R(x_orig \<mapsto> x2)) (update_var \<Lambda> ns x_orig v) ?U'")
+               \<Lambda> \<Lambda>' (R(x_orig \<mapsto> (Inl x2))) (update_var \<Lambda> ns x_orig v) ?U'")
   using assms
   unfolding nstate_rel_states_def
   by (simp add: update_var_nstate_rel)  
@@ -523,20 +546,23 @@ definition passive_sim
                        (\<forall>ns'. s' = Normal ns' \<longrightarrow> (su = Normal u \<and> nstate_rel \<Lambda> \<Lambda>' R ns' u \<and> rel_well_typed A \<Lambda> \<Omega> R ns')))"
 
 
-inductive passive_cmds_rel :: "vname list \<Rightarrow> (vname \<rightharpoonup> vname) \<Rightarrow> (vname \<times> vname) list \<Rightarrow> cmd list \<Rightarrow> cmd list \<Rightarrow> bool"
+inductive passive_cmds_rel :: "vname list \<Rightarrow> passive_rel \<Rightarrow> (vname \<times> (vname + lit)) list \<Rightarrow> cmd list \<Rightarrow> cmd list \<Rightarrow> bool"
   where 
     PAssignNormal: 
-    "\<lbrakk> expr_rel R e1 e2; passive_cmds_rel W (R(x1 \<mapsto> x2)) Q cs1 cs2 \<rbrakk> \<Longrightarrow> 
-        passive_cmds_rel (x2#W) R ((x1,x2)#Q) ((Assign x1 e1) # cs1) ((Assume ((Var x2) \<guillemotleft>Eq\<guillemotright> e2)) # cs2)"
+    "\<lbrakk> expr_rel R e1 e2; passive_cmds_rel W (R(x1 \<mapsto> (Inl x2))) Q cs1 cs2 \<rbrakk> \<Longrightarrow> 
+        passive_cmds_rel (x2#W) R ((x1,(Inl x2))#Q) ((Assign x1 e1) # cs1) ((Assume ((Var x2) \<guillemotleft>Eq\<guillemotright> e2)) # cs2)"
   | PAssert: 
-    "\<lbrakk> expr_rel R e1 e2; passive_cmds_rel W R Q cs1 cs2 \<rbrakk> \<Longrightarrow> passive_cmds_rel W R Q ((Assert e1) # cs1) ((Assert e2) # cs2)"
+    "\<lbrakk> expr_rel R e1 e2; passive_cmds_rel W R Q cs1 cs2 \<rbrakk> \<Longrightarrow> 
+        passive_cmds_rel W R Q ((Assert e1) # cs1) ((Assert e2) # cs2)"
   | PAssumeNormal: 
-    "\<lbrakk> expr_rel R e1 e2; passive_cmds_rel W R Q cs1 cs2 \<rbrakk> \<Longrightarrow> passive_cmds_rel W R Q ((Assume e1) # cs1) ((Assume e2) # cs2)"
+    "\<lbrakk> expr_rel R e1 e2; passive_cmds_rel W R Q cs1 cs2 \<rbrakk> \<Longrightarrow> 
+        passive_cmds_rel W R Q ((Assume e1) # cs1) ((Assume e2) # cs2)"
   | PHavoc: 
-    "\<lbrakk> passive_cmds_rel W (R(x \<mapsto> x')) Q cs1 cs2\<rbrakk> \<Longrightarrow> passive_cmds_rel (x'#W) R ((x,x')#Q) ((Havoc x) # cs1) cs2"
+    "\<lbrakk> passive_cmds_rel W (R(x \<mapsto> (Inl x'))) Q cs1 cs2\<rbrakk> \<Longrightarrow> 
+       passive_cmds_rel (x'#W) R ((x,(Inl x'))#Q) ((Havoc x) # cs1) cs2"
   | PSync:       
-    "\<lbrakk> R x = Some x1; passive_cmds_rel W (R(x \<mapsto> x2)) Q [] cs \<rbrakk> \<Longrightarrow>
-                passive_cmds_rel (x2#W) R ((x,x2)#Q) [] ((Assume ( (Var x2) \<guillemotleft>Eq\<guillemotright> (Var x1))) # cs)"
+    "\<lbrakk> R x = Some (Inl x1); passive_cmds_rel W (R(x \<mapsto> (Inl x2))) Q [] cs \<rbrakk> \<Longrightarrow>
+       passive_cmds_rel (x2#W) R ((x,(Inl x2))#Q) [] ((Assume ( (Var x2) \<guillemotleft>Eq\<guillemotright> (Var x1))) # cs)"
   | PNil: "passive_cmds_rel [] R [] [] []"
 
 method passive_rel_tac uses R_def = 
@@ -563,8 +589,12 @@ lemma
   oops
 *)
 
-definition type_rel :: "var_context \<Rightarrow> var_context \<Rightarrow> (vname \<times> vname) list \<Rightarrow> bool"
-  where "type_rel \<Lambda> \<Lambda>' Q = list_all (\<lambda> t. lookup_var_ty \<Lambda> (fst t) = lookup_var_ty \<Lambda>' (snd t)) Q"
+definition type_rel :: "var_context \<Rightarrow> var_context \<Rightarrow> (vname \<times> (vname + lit)) list \<Rightarrow> bool"
+  where "type_rel \<Lambda> \<Lambda>' Q = list_all (\<lambda> t. 
+                case (snd t) of
+                 (Inl y) \<Rightarrow>  lookup_var_ty \<Lambda> (fst t) = lookup_var_ty \<Lambda>' y 
+                | (Inr _) \<Rightarrow> True
+                  ) Q"
 
   
 (* helper lemma to prove semantic block lemma *)
@@ -590,13 +620,13 @@ lemma passification_block_lemma_aux:
 proof (induction arbitrary: ns U0 D0)
   case (PAssignNormal R e1 e2 W x1 x2 Q cs1 cs2)
   (* TODO: share proof with case PSync *)
-  hence "x2 \<notin> D0" by simp
+  hence "x2 \<notin> D0" and "rel_const_correct \<Lambda> R ns" by (auto simp: rel_well_typed_def)
   from \<open>A,M,\<Lambda>,\<Gamma>,\<Omega> \<turnstile> \<langle>Assign x1 e1 # cs1,Normal ns\<rangle> [\<rightarrow>] s'\<close> obtain v1 \<tau>
     where RedE1:"A,\<Lambda>,\<Gamma>,\<Omega> \<turnstile> \<langle>e1,ns\<rangle> \<Down> v1" and LookupX1:"lookup_var_ty \<Lambda> x1 = Some \<tau>" and 
                 TyV1:"type_of_val A v1 = instantiate \<Omega> \<tau>" by (meson RedCmdListCons_case single_assign_reduce_2)
-  with expr_rel_same_set[OF \<open>expr_rel R e1 e2\<close> _ \<open>nstate_rel_states \<Lambda> \<Lambda>' R ns U0\<close>]
+  with expr_rel_same_set[OF \<open>expr_rel R e1 e2\<close> _ \<open>rel_const_correct \<Lambda> R ns\<close> \<open>nstate_rel_states \<Lambda> \<Lambda>' R ns U0\<close>]
   have RedE2:"\<forall>u\<in>U0. A, \<Lambda>',\<Gamma>,\<Omega> \<turnstile> \<langle>e2,u\<rangle> \<Down> v1" by blast  
-  from LookupX1 have LookupX2:"lookup_var_ty \<Lambda>' x2 = Some \<tau>" using \<open>type_rel \<Lambda> \<Lambda>' ((x1, x2) # Q)\<close> by (simp add: type_rel_def)
+  from LookupX1 have LookupX2:"lookup_var_ty \<Lambda>' x2 = Some \<tau>" using \<open>type_rel \<Lambda> \<Lambda>' ((x1, (Inl x2)) # Q)\<close> by (simp add: type_rel_def)
   let ?U1 = "(set_red_cmd A M \<Lambda>' \<Gamma> \<Omega> (Assume ((Var x2) \<guillemotleft>Eq\<guillemotright> e2)) U0)"
   let ?U1Normal = "{ns. Normal ns \<in> ?U1}"   
   have U1Sub:"?U1Normal \<subseteq> U0"
@@ -605,16 +635,16 @@ proof (induction arbitrary: ns U0 D0)
     by (blast dest: assume_assign_non_empty)
   have U1Dep: "dependent A \<Lambda>' \<Omega> ?U1Normal (D0 \<union> {x2})" using \<open>x2 \<notin> D0\<close> \<open>dependent A \<Lambda>' \<Omega> U0 D0\<close> RedE2    
     by (blast dest:  assume_assign_dependent)
-    have RelStates: "nstate_rel_states \<Lambda> \<Lambda>' (R(x1 \<mapsto> x2)) (update_var \<Lambda> ns x1 v1) ?U1Normal"
-      using \<open>nstate_rel_states \<Lambda> \<Lambda>' R ns U0\<close> \<open>expr_rel R e1 e2\<close> RedE1
+    have RelStates: "nstate_rel_states \<Lambda> \<Lambda>' (R(x1 \<mapsto> (Inl x2))) (update_var \<Lambda> ns x1 v1) ?U1Normal"
+      using \<open>nstate_rel_states \<Lambda> \<Lambda>' R ns U0\<close> \<open>expr_rel R e1 e2\<close> \<open>rel_const_correct \<Lambda> R ns\<close> RedE1
       by (blast dest: assume_assign_nstate_rel)
   from \<open>distinct (x2 # W)\<close> \<open>set (x2 # W) \<inter> D0 = {}\<close> have "distinct W" and "set W \<inter> (D0 \<union> {x2}) = {}" by auto
   from \<open>A,M,\<Lambda>,\<Gamma>,\<Omega> \<turnstile> \<langle>Assign x1 e1 # cs1,Normal ns\<rangle> [\<rightarrow>] s'\<close> have RedCs1:\<open>A,M,\<Lambda>,\<Gamma>,\<Omega> \<turnstile> \<langle>cs1, Normal (update_var \<Lambda> ns x1 v1)\<rangle> [\<rightarrow>] s'\<close>
     by (metis RedCmdListCons_case RedE1 expr_eval_determ(1) single_assign_cases)
   have RedAssume: "\<And>u. u \<in> ?U1Normal \<Longrightarrow> A,M,\<Lambda>',\<Gamma>,\<Omega> \<turnstile> \<langle>Assume ((Var x2) \<guillemotleft>Eq\<guillemotright> e2),Normal u\<rangle> \<rightarrow> Normal u"    
     by (rule passive_states_propagate_2) simp
-  from \<open>type_rel \<Lambda> \<Lambda>' ((x1, x2) # Q)\<close> have QTyRel:"type_rel \<Lambda> \<Lambda>' Q" by (simp add: type_rel_def)
-  from \<open>rel_well_typed A \<Lambda> \<Omega> R ns\<close> have Rel_wt:\<open>rel_well_typed A \<Lambda> \<Omega> (R(x1 \<mapsto> x2)) (update_var \<Lambda> ns x1 v1)\<close> using LookupX1 TyV1    
+  from \<open>type_rel \<Lambda> \<Lambda>' ((x1, (Inl x2)) # Q)\<close> have QTyRel:"type_rel \<Lambda> \<Lambda>' Q" by (simp add: type_rel_def)
+  from \<open>rel_well_typed A \<Lambda> \<Omega> R ns\<close> have Rel_wt:\<open>rel_well_typed A \<Lambda> \<Omega> (R(x1 \<mapsto> (Inl x2))) (update_var \<Lambda> ns x1 v1)\<close> using LookupX1 TyV1    
     by (blast dest: rel_well_typed_update)
   from PAssignNormal.IH[OF RedCs1 U1Dep RelStates Rel_wt \<open>set W \<inter> (D0 \<union> {x2}) = {}\<close>  U1NonEmpty QTyRel \<open>distinct W\<close>] obtain U2 where
     U2Sub:"U2 \<subseteq> ?U1Normal" and
@@ -622,7 +652,7 @@ proof (induction arbitrary: ns U0 D0)
     U2Rel:"(\<forall>u\<in>U2.
          \<exists>su. (A,M,\<Lambda>',\<Gamma>,\<Omega> \<turnstile> \<langle>cs2,Normal u\<rangle> [\<rightarrow>] su) \<and>
               (s' = Failure \<longrightarrow> su = Failure) \<and> 
-              (\<forall>ns'. s' = Normal ns' \<longrightarrow> su = Normal u \<and> nstate_rel \<Lambda> \<Lambda>' (update_nstate_rel (R(x1 \<mapsto> x2)) Q) ns' u \<and> rel_well_typed A \<Lambda> \<Omega> (update_nstate_rel (R(x1 \<mapsto> x2)) Q) ns'))"
+              (\<forall>ns'. s' = Normal ns' \<longrightarrow> su = Normal u \<and> nstate_rel \<Lambda> \<Lambda>' (update_nstate_rel (R(x1 \<mapsto> (Inl x2))) Q) ns' u \<and> rel_well_typed A \<Lambda> \<Omega> (update_nstate_rel (R(x1 \<mapsto> (Inl x2))) Q) ns'))"
     by blast
   hence U2Sub':"U2 \<subseteq> U0" and  U2Dep':"dependent A \<Lambda>' \<Omega> U2 (D0 \<union> set (x2 # W))" and 
         RedAssume2:"\<And>u. u \<in> U2 \<Longrightarrow> A,M,\<Lambda>',\<Gamma>,\<Omega> \<turnstile> \<langle>Assume ((Var x2) \<guillemotleft>Eq\<guillemotright> e2),Normal u\<rangle> \<rightarrow> Normal u" using U1Sub RedAssume by auto
@@ -632,6 +662,7 @@ proof (induction arbitrary: ns U0 D0)
      by (metis RedCmdListCons)
 next
   case (PAssert R e1 e2 W Q cs1 cs2)
+  hence "rel_const_correct \<Lambda> R ns" by (simp add: rel_well_typed_def)
   from \<open>A,M,\<Lambda>,\<Gamma>,\<Omega> \<turnstile> \<langle>Assert e1 # cs1,Normal ns\<rangle> [\<rightarrow>] s'\<close> obtain s'' where 
     RedAssert:"A,M,\<Lambda>,\<Gamma>,\<Omega> \<turnstile> \<langle>Assert e1,Normal ns\<rangle> \<rightarrow> s''" and
     RedCs1:"A,M,\<Lambda>,\<Gamma>,\<Omega> \<turnstile> \<langle>cs1, s''\<rangle> [\<rightarrow>] s'" 
@@ -640,7 +671,7 @@ next
   proof cases
     case RedAssertOk
     hence RedE2:"\<And>u. u\<in>U0 \<Longrightarrow> A,M,\<Lambda>',\<Gamma>,\<Omega> \<turnstile> \<langle>Assert e2,Normal u\<rangle> \<rightarrow> Normal u"
-      using assert_rel_normal_2 \<open>nstate_rel_states \<Lambda> \<Lambda>' R ns U0\<close> \<open>expr_rel R e1 e2\<close> by blast
+      using assert_rel_normal_2 \<open>nstate_rel_states \<Lambda> \<Lambda>' R ns U0\<close> \<open>expr_rel R e1 e2\<close> \<open>rel_const_correct \<Lambda> R ns\<close> by blast
     from \<open>s'' = Normal ns\<close> RedCs1 have RedCs1Normal:"A,M,\<Lambda>,\<Gamma>,\<Omega> \<turnstile> \<langle>cs1, Normal ns\<rangle> [\<rightarrow>] s'" by simp
     from PAssert.IH[OF RedCs1Normal \<open>dependent A \<Lambda>' \<Omega> U0 D0\<close>] obtain U1 
       where U1Sub: "U1 \<subseteq> U0" and "U1 \<noteq> {}" and U1Dep:"dependent A \<Lambda>' \<Omega> U1 (D0 \<union> set W)" and
@@ -659,7 +690,7 @@ next
   next
     case RedAssertFail
     hence RedE2:"\<And>u. u\<in>U0 \<Longrightarrow> A,M,\<Lambda>',\<Gamma>,\<Omega> \<turnstile> \<langle>Assert e2,Normal u\<rangle> \<rightarrow> Failure" 
-      using assert_rel_failure \<open>nstate_rel_states \<Lambda> \<Lambda>' R ns U0\<close> \<open>expr_rel R e1 e2\<close> by blast
+      using assert_rel_failure \<open>nstate_rel_states \<Lambda> \<Lambda>' R ns U0\<close> \<open>expr_rel R e1 e2\<close> \<open>rel_const_correct \<Lambda> R ns\<close> by blast
     from  \<open>s'' = Failure\<close> have "s' = Failure" using RedCs1
       by (simp add: failure_stays_cmd_list)
     show ?thesis
@@ -671,6 +702,7 @@ next
   qed
 next
   case (PAssumeNormal R e1 e2 W Q cs1 cs2)
+  hence "rel_const_correct \<Lambda> R ns" by (simp add: rel_well_typed_def)
   from \<open>A,M,\<Lambda>,\<Gamma>,\<Omega> \<turnstile> \<langle>Assume e1 # cs1,Normal ns\<rangle> [\<rightarrow>] s'\<close> obtain s'' where 
     RedAssume:"A,M,\<Lambda>,\<Gamma>,\<Omega> \<turnstile> \<langle>Assume e1,Normal ns\<rangle> \<rightarrow> s''" and
     RedCs1:"A,M,\<Lambda>,\<Gamma>,\<Omega> \<turnstile> \<langle>cs1, s''\<rangle> [\<rightarrow>] s'" 
@@ -679,7 +711,7 @@ next
   proof cases
     case RedAssumeOk
     hence RedE2:"\<And>u. u\<in>U0 \<Longrightarrow> A,M,\<Lambda>',\<Gamma>,\<Omega> \<turnstile> \<langle>Assume e2,Normal u\<rangle> \<rightarrow> Normal u"
-      using assume_rel_normal \<open>nstate_rel_states \<Lambda> \<Lambda>' R ns U0\<close> \<open>expr_rel R e1 e2\<close> by blast
+      using assume_rel_normal \<open>nstate_rel_states \<Lambda> \<Lambda>' R ns U0\<close> \<open>expr_rel R e1 e2\<close> \<open>rel_const_correct \<Lambda> R ns\<close> by blast
     from \<open>s'' = Normal ns\<close> RedCs1 have RedCs1Normal:"A,M,\<Lambda>,\<Gamma>,\<Omega> \<turnstile> \<langle>cs1, Normal ns\<rangle> [\<rightarrow>] s'" by simp
     from PAssumeNormal.IH[OF RedCs1Normal \<open>dependent A \<Lambda>' \<Omega> U0 D0\<close>] obtain U1 
       where U1Sub: "U1 \<subseteq> U0" and "U1 \<noteq> {}" and U1Dep:"dependent A \<Lambda>' \<Omega> U1 (D0 \<union> set W)" and
@@ -698,7 +730,7 @@ next
   next
     case RedAssumeMagic
     hence  RedE2:"\<And>u. u\<in>U0 \<Longrightarrow> A,M,\<Lambda>',\<Gamma>,\<Omega> \<turnstile> \<langle>Assume e2,Normal u\<rangle> \<rightarrow> Magic"
-      using assume_rel_magic \<open>nstate_rel_states \<Lambda> \<Lambda>' R ns U0\<close> \<open>expr_rel R e1 e2\<close> by blast
+      using assume_rel_magic \<open>nstate_rel_states \<Lambda> \<Lambda>' R ns U0\<close> \<open>expr_rel R e1 e2\<close> \<open>rel_const_correct \<Lambda> R ns\<close> by blast
     from \<open>s'' = Magic\<close> have "s' = Magic" using RedCs1
       by (simp add: magic_stays_cmd_list) 
     show ?thesis 
@@ -714,17 +746,17 @@ next
     RedCs1:"A,M,\<Lambda>,\<Gamma>,\<Omega> \<turnstile> \<langle>cs1,Normal (update_var \<Lambda> ns x v)\<rangle> [\<rightarrow>] s'" and 
     LookupX:"lookup_var_ty \<Lambda> x = Some \<tau>" and TyV:"type_of_val A v = instantiate \<Omega> \<tau>"
     by (blast elim: havoc_cases_2)
-  hence LookupX':"lookup_var_ty \<Lambda>' x' = Some \<tau>" using \<open>type_rel \<Lambda> \<Lambda>' ((x, x') # Q)\<close> by (simp add: type_rel_def)
+  hence LookupX':"lookup_var_ty \<Lambda>' x' = Some \<tau>" using \<open>type_rel \<Lambda> \<Lambda>' ((x, (Inl x')) # Q)\<close> by (simp add: type_rel_def)
   let ?U1 = "{u' \<in> U0. lookup_var \<Lambda>' u' x' = Some v}"
   have DepU1:"dependent A \<Lambda>' \<Omega> ?U1 (D0 \<union> {x'})" and  "?U1 \<noteq> {}"
     using \<open>dependent A \<Lambda>' \<Omega> U0 D0\<close> \<open>x' \<notin> D0\<close> \<open>U0 \<noteq> {}\<close> LookupX' TyV
    by (blast dest: havoc_dependent havoc_non_empty)+
 
-  have RelU1:"nstate_rel_states \<Lambda> \<Lambda>' (R(x \<mapsto> x')) (update_var \<Lambda> ns x v) ?U1" using \<open>nstate_rel_states \<Lambda> \<Lambda>' R ns U0\<close>
+  have RelU1:"nstate_rel_states \<Lambda> \<Lambda>' (R(x \<mapsto> (Inl x'))) (update_var \<Lambda> ns x v) ?U1" using \<open>nstate_rel_states \<Lambda> \<Lambda>' R ns U0\<close>
     by (blast dest: havoc_nstate_rel)
   have U1Sub: "?U1 \<subseteq> U0" by auto
-  from \<open>type_rel \<Lambda> \<Lambda>' ((x, x') # Q)\<close> have QTyRel:"type_rel \<Lambda> \<Lambda>' Q" by (simp add: type_rel_def)
-  from \<open>rel_well_typed A \<Lambda> \<Omega> R ns\<close> have Rel_wt:\<open>rel_well_typed A \<Lambda> \<Omega> (R(x \<mapsto> x')) (update_var \<Lambda> ns x v)\<close>
+  from \<open>type_rel \<Lambda> \<Lambda>' ((x, Inl x') # Q)\<close> have QTyRel:"type_rel \<Lambda> \<Lambda>' Q" by (simp add: type_rel_def)
+  from \<open>rel_well_typed A \<Lambda> \<Omega> R ns\<close> have Rel_wt:\<open>rel_well_typed A \<Lambda> \<Omega> (R(x \<mapsto> Inl x')) (update_var \<Lambda> ns x v)\<close>
     using LookupX TyV    
     by (blast dest: rel_well_typed_update)
   from PHavoc.IH[OF RedCs1 DepU1 RelU1 Rel_wt Disj \<open>?U1 \<noteq> {}\<close> QTyRel \<open>distinct W\<close>] obtain U2 where
@@ -733,7 +765,7 @@ next
        "(\<forall>u\<in>U2.
          \<exists>su. (A,M,\<Lambda>',\<Gamma>,\<Omega> \<turnstile> \<langle>cs2,Normal u\<rangle> [\<rightarrow>] su) \<and>
               (s' = Failure \<longrightarrow> su = Failure) \<and>
-              (\<forall>ns'. s' = Normal ns' \<longrightarrow> su = Normal u \<and> nstate_rel \<Lambda> \<Lambda>' (update_nstate_rel (R(x \<mapsto> x')) Q) ns' u \<and> rel_well_typed A \<Lambda> \<Omega> (update_nstate_rel (R(x \<mapsto> x')) Q) ns'))"
+              (\<forall>ns'. s' = Normal ns' \<longrightarrow> su = Normal u \<and> nstate_rel \<Lambda> \<Lambda>' (update_nstate_rel (R(x \<mapsto> Inl x')) Q) ns' u \<and> rel_well_typed A \<Lambda> \<Omega> (update_nstate_rel (R(x \<mapsto> Inl x')) Q) ns'))"
     by blast 
   thus ?case    
     apply (simp)
@@ -750,24 +782,24 @@ next
   let ?U1Normal = "{ns. Normal ns \<in> ?U1}"   
   have U1Sub:"?U1Normal \<subseteq> U0"
     by (simp add: passive_states_subset)
-  from \<open>R x = Some x1\<close> \<open>rel_well_typed A \<Lambda> \<Omega> R ns\<close> obtain v \<tau> where 
+  from \<open>R x = Some (Inl x1)\<close> \<open>rel_well_typed A \<Lambda> \<Omega> R ns\<close> obtain v \<tau> where 
        LookupX:"lookup_var \<Lambda> ns x = Some v" and LookupTy:"lookup_var_ty \<Lambda> x = Some \<tau>" and TyV:"type_of_val A v = instantiate \<Omega> \<tau>" 
        by (auto simp: rel_well_typed_def)
   hence RedX1:"\<forall>u\<in>U0. A,\<Lambda>',\<Gamma>,\<Omega> \<turnstile> \<langle>Var x1,u\<rangle> \<Down> v"        
-    using \<open>nstate_rel_states \<Lambda> \<Lambda>' R ns U0\<close> \<open>R x = Some x1\<close> \<open>rel_well_typed A \<Lambda> \<Omega> R ns\<close> by (fastforce dest: lookup_nstates_rel intro: RedVar)
-  from LookupTy have "lookup_var_ty \<Lambda>' x2 = Some \<tau>" using \<open>type_rel \<Lambda> \<Lambda>' ((x, x2) # Q)\<close> by (simp add: type_rel_def)
+    using \<open>nstate_rel_states \<Lambda> \<Lambda>' R ns U0\<close> \<open>R x = Some (Inl x1)\<close> \<open>rel_well_typed A \<Lambda> \<Omega> R ns\<close> by (fastforce dest: lookup_nstates_rel intro: RedVar)
+  from LookupTy have "lookup_var_ty \<Lambda>' x2 = Some \<tau>" using \<open>type_rel \<Lambda> \<Lambda>' ((x, Inl x2) # Q)\<close> by (simp add: type_rel_def)
   hence U1NonEmpty: "?U1Normal \<noteq> {}" using RedX1 \<open>U0 \<noteq> {}\<close> \<open>dependent A \<Lambda>' \<Omega> U0 D0\<close> \<open>x2 \<notin> D0\<close> TyV
     using  assume_assign_non_empty by (blast dest: assume_assign_non_empty)
   have U1Dep: "dependent A \<Lambda>' \<Omega> ?U1Normal (D0 \<union> {x2})"
     using \<open>dependent A \<Lambda>' \<Omega> U0 D0\<close> \<open>x2 \<notin> D0\<close> RedX1
     by (blast dest: assume_assign_dependent)
-  have RelStates: "nstate_rel_states \<Lambda> \<Lambda>' (R(x \<mapsto> x2)) ns ?U1Normal" 
-    using \<open>nstate_rel_states \<Lambda> \<Lambda>' R ns U0\<close>  \<open>R x = Some x1\<close> \<open>rel_well_typed A \<Lambda> \<Omega> R ns\<close> by (blast dest: assume_sync_nstate_rel)
+  have RelStates: "nstate_rel_states \<Lambda> \<Lambda>' (R(x \<mapsto> Inl x2)) ns ?U1Normal" 
+    using \<open>nstate_rel_states \<Lambda> \<Lambda>' R ns U0\<close>  \<open>R x = Some (Inl x1)\<close> \<open>rel_well_typed A \<Lambda> \<Omega> R ns\<close> by (blast dest: assume_sync_nstate_rel)
   have RedAssume: "\<And>u. u \<in> ?U1Normal \<Longrightarrow> A,M,\<Lambda>',\<Gamma>,\<Omega> \<turnstile> \<langle>Assume ((Var x2) \<guillemotleft>Eq\<guillemotright> (Var x1)),Normal u\<rangle> \<rightarrow> Normal u"    
     by (rule passive_states_propagate_2) simp
   from \<open>distinct (x2 # W)\<close> \<open>set (x2 # W) \<inter> D0 = {}\<close> have "distinct W" and "set W \<inter> (D0 \<union> {x2}) = {}" by auto
-  from \<open>type_rel \<Lambda> \<Lambda>' ((x, x2) # Q)\<close> have QTyRel:"type_rel \<Lambda> \<Lambda>' Q" by (simp add: type_rel_def)
-  from \<open>rel_well_typed A \<Lambda> \<Omega> R ns\<close> have Rel_wt:\<open>rel_well_typed A \<Lambda> \<Omega> (R(x \<mapsto> x2)) ns\<close> using \<open>R x = Some x1\<close> by (simp add: rel_well_typed_def)
+  from \<open>type_rel \<Lambda> \<Lambda>' ((x, (Inl x2)) # Q)\<close> have QTyRel:"type_rel \<Lambda> \<Lambda>' Q" by (simp add: type_rel_def)
+  from \<open>rel_well_typed A \<Lambda> \<Omega> R ns\<close> have Rel_wt:\<open>rel_well_typed A \<Lambda> \<Omega> (R(x \<mapsto> (Inl x2))) ns\<close> using \<open>R x = Some (Inl x1)\<close> by (simp add: rel_well_typed_def rel_const_correct_def)
   from PSync.IH[OF \<open>A,M,\<Lambda>,\<Gamma>,\<Omega> \<turnstile> \<langle>[],Normal ns\<rangle> [\<rightarrow>] s'\<close> U1Dep RelStates Rel_wt \<open>set W \<inter> (D0 \<union> {x2}) = {}\<close> U1NonEmpty QTyRel \<open>distinct W\<close>]
   obtain U2 where 
       U2Sub:"U2 \<subseteq> ?U1Normal" and
@@ -776,7 +808,7 @@ next
         "\<forall>u\<in>U2.
          \<exists>su. (A,M,\<Lambda>',\<Gamma>,\<Omega> \<turnstile> \<langle>cs,Normal u\<rangle> [\<rightarrow>] su) \<and>
               (s' = Failure \<longrightarrow> su = Failure) \<and> (\<forall>ns'. s' = Normal ns' \<longrightarrow> su = Normal u \<and>
-              nstate_rel \<Lambda> \<Lambda>' (update_nstate_rel (R(x \<mapsto> x2)) Q) ns' u \<and> rel_well_typed A \<Lambda> \<Omega> (update_nstate_rel (R(x \<mapsto> x2)) Q) ns')"
+              nstate_rel \<Lambda> \<Lambda>' (update_nstate_rel (R(x \<mapsto> Inl x2)) Q) ns' u \<and> rel_well_typed A \<Lambda> \<Omega> (update_nstate_rel (R(x \<mapsto> Inl x2)) Q) ns')"
     by blast
   hence U2Sub':"U2 \<subseteq> U0" and  U2Dep':"dependent A \<Lambda>' \<Omega> U2 (D0 \<union> set (x2 # W))" and 
     RedAssume2:"\<And>u. u \<in> U2 \<Longrightarrow> A,M,\<Lambda>',\<Gamma>,\<Omega> \<turnstile> \<langle>Assume ((Var x2) \<guillemotleft>Eq\<guillemotright> (Var x1)),Normal u\<rangle> \<rightarrow> Normal u"
@@ -795,23 +827,50 @@ definition passive_block_conclusion
   where "passive_block_conclusion A M \<Lambda> \<Lambda>' \<Gamma> \<Omega> U0 D1 R cs2 s' = 
   (\<exists> U1 \<subseteq> U0. U1 \<noteq> {} \<and> dependent A \<Lambda>' \<Omega> U1 D1 \<and> passive_sim A M \<Lambda> \<Lambda>' \<Gamma> \<Omega> cs2 s' R U1)"
 
-definition passive_block_assms
-  where "passive_block_assms A M \<Lambda> \<Lambda>' \<Gamma> \<Omega> W R U0 D0 cs1 ns s' = 
+definition passive_lemma_assms
+  where "passive_lemma_assms A M \<Lambda> \<Lambda>' \<Gamma> \<Omega> W R U0 D0 cs1 ns s' = 
           (nstate_rel_states \<Lambda> \<Lambda>' R ns U0 \<and> rel_well_typed A \<Lambda> \<Omega> R ns \<and>
-          (A,M,\<Lambda>,\<Gamma>,\<Omega> \<turnstile> \<langle>cs1, Normal ns\<rangle> [\<rightarrow>] s') \<and> dependent A \<Lambda>' \<Omega> U0 D0 \<and> (set W) \<inter> D0 = {} \<and>
+          dependent A \<Lambda>' \<Omega> U0 D0 \<and> (set W) \<inter> D0 = {} \<and>
           U0 \<noteq> {})"
-
-text \<open>\<open>passive_cmds_rel W R Q cs1 cs2\<close> passive_cmds_rel and \<open>distinct W\<close> must be proved for the final block lemma\<close>
 
 lemma passification_block_lemma_compact:
   assumes 
-          "passive_block_assms A M \<Lambda> \<Lambda>' \<Gamma> \<Omega> W R U0 D0 cs1 ns s'" and
+          "A,M,\<Lambda>,\<Gamma>,\<Omega> \<turnstile> \<langle>cs1, Normal ns\<rangle> [\<rightarrow>] s'"
+          "passive_lemma_assms A M \<Lambda> \<Lambda>' \<Gamma> \<Omega> W R U0 D0 cs1 ns s'" and
           "passive_cmds_rel W R Q cs1 cs2" and
           "type_rel \<Lambda> \<Lambda>' Q" and
           "distinct W"
   shows "passive_block_conclusion A M \<Lambda> \<Lambda>' \<Gamma> \<Omega> U0 (D0 \<union> (set W)) (update_nstate_rel R Q) cs2 s'"
   using assms
-  unfolding passive_block_assms_def passive_block_conclusion_def
+  unfolding passive_lemma_assms_def passive_block_conclusion_def
   using passification_block_lemma_aux by meson
+
+text \<open>CFG proofs\<close>
+definition passive_cfg_assms
+  where "passive_cfg_assms A M \<Lambda> \<Lambda>' \<Gamma> \<Omega> G W R U0 D0 m m' ns s' = 
+          ( (A,M,\<Lambda>,\<Gamma>,\<Omega>,G \<turnstile> (m, Normal ns) -n\<rightarrow>* (m',s')) \<and>
+           nstate_rel_states \<Lambda> \<Lambda>' R ns U0 \<and> rel_well_typed A \<Lambda> \<Omega> R ns \<and>
+           dependent A \<Lambda>' \<Omega> U0 D0 \<and> (set W) \<inter> D0 = {} \<and>
+          U0 \<noteq> {})"
+
+definition passive_sim_cfg
+  where "passive_sim_cfg A M \<Lambda>' \<Gamma> \<Omega> G U m_p s' \<equiv> 
+              (\<forall>u \<in> U. \<exists> m_p' su. (A,M,\<Lambda>',\<Gamma>,\<Omega>, G \<turnstile> (m_p, Normal u) -n\<rightarrow>* (m_p',su)) \<and> 
+                       (s' = Failure \<longrightarrow> su = Failure))"
+
+(*
+definition passive_cfg_conclusion
+  where "passive_cfg_conclusion A M \<Lambda> \<Lambda>' \<Gamma> \<Omega> G U0 D1 R m m' s' = 
+  (\<exists> U1 \<subseteq> U0. U1 \<noteq> {} \<and> dependent A \<Lambda>' \<Omega> U1 D1 \<and> passive_sim_cfg A M \<Lambda>' \<Gamma> \<Omega> G U1 m m' s')"
+
+definition passive_cfg_lemma
+  where "passive_cfg_lemma A M \<Lambda> \<Lambda>' \<Gamma> \<Omega> G W R U0 D0 m m' m_p m_p' ns s' =
+          (passive_cfg_assms A M \<Lambda> \<Lambda>' \<Gamma> \<Omega> G W R U0 D0 m m' ns s' \<longrightarrow>
+           passive_cfg_conclusion A M \<Lambda> \<Lambda>' \<Gamma> \<Omega> G U0 (D0 \<union> (set W)) R m_p m_p' s')"
+*)
+
+  
+          
+          
 
 end
